<!-- S → A | ɛ
A → 0 | 1 | A+A | ɛ | AA | (A) | A*


**better**
S → A | C | D | F
A → 0 | 1 | AA | D | C
C → A+A
D → (A)
F → A* | C* | D*


V1
S → A
A → 0 | 1 | D | C | F | 0* | 1* | e
D → (D) | (D)* | A
C → C+C | A
F → AA

Refined: -->
The required CFG as follows:
R → A | $\phi$
A → 0 | 1 | $\epsilon$ | D | C | F | 0* | 1* 
D → (D) | (D)* | A
C → C+C | A
F → AA

*   So G = (V,T,R,S) where
    *   V = {R,A,B,C,D,F}
    *   T = {0, 1, (, ), +,∗, $\epsilon$, ∅}
    *   R = {S → A | $\phi$,
        A → 0 | 1 | $\epsilon$ | D | C | F | 0* | 1*, 
        D → (D) | (D)* | A,
        C → C+C | A,
        F → AA }
    *   S = {R} (the variable to the left of first arrow)