$S \rightarrow 0S0$ (Rule 1)
$S \rightarrow 0S1S0$ (Rule 2)
$S \rightarrow \epsilon$ (Rule 3)

W = 0001000
Using leftmost derivation:
<!-- Derivation 1:
| Rule No | Rule      | Application | Result   |
| ------- | --------- | ----------- | -------- |
| 2       | S → 0S1S0 | S           | 0S1S0    |
| 1       | S → 0S0   | 0S1S0       | 00S01S0  |
| 3       | S → ɛ     | 00S01S0     | 0001S0   |
| 1       | S → 0S0   | 0001S0      | 00010S00 |
| 3       | S → ɛ     | 00010S00    | 0001000  | -->

Derivation 1 :
S $=>^2$ 0S1S0 $=>^1$ 00S01S0 $=>^3$ 0001S0 $=>^1$ 00010S00 $=>^3$ 0001000


<!-- Derivation 2: 
| Rule No | Rule      | Application | Result    |
| ------- | --------- | ----------- | --------- |
| 1       | S → 0S0   | S           | 0S0       |
| 1       | S → 0S0   | 0S0         | 00S00     |
| 2       | S → 0S1S0 | 00S00       | 000S1S000 |
| 3       | S → ɛ     | 000S1S000   | 0001S000  |
| 3       | S → ɛ     | 0001S000    | 0001000   | -->
Derivation 2 :
S $=>^1$ 0S0 $=>^1$ 00S00 $=>^2$000S1S000 $=>^3$ 0001S000 $=>^3$ 0001000