- [a](#a)
- [b](#b)
- [c](#c)
# a
- Oponent chooses, p
- We choose, $W = 0^p1^p$
- Oponent chooses, XYZ
- 
# b
- Oponent chooses, p
- We choose, W = $1^p1011^p$ 
  - since, k = p+1, $k\geq 1$,  
$U = 011^p$, $\#_1(U) = p+1$, and $\#_1(U) = k$, 
therefore  $W \in L$
- Opponet chooses, 
  - $X = 1^a$
  - $Y = 1^b$
  - $XY = 1^a\cdot 1^b$ where $a+b\leq p$ and $b>0$
  - $XYZ = 1^a\cdot 1^b\cdot 1^{p+1-(a+b)} \cdot 0\cdot 1\cdot 1^p$
- We choose, $y^0$, 
  - hence $W' = XY^0Z = 1^a\cdot 1^{p+1-(a+b)} \cdot 0\cdot 1\cdot1^p$
  $\therefore$ $W' = 1^{a+p+1-a-b}\cdot0\cdot 1\cdot1^p = 1^{p+1-b}\cdot0\cdot 1\cdot1^p$
  $\implies$, $k = p+1-b$, $U = 011^p$ and $\#_1(U) = p+1$
  Since $b>0$ 
  $\therefore p+1 > p+1-b\implies \#_1(U)>k$
  $\therefore$ $W' \notin L$



# c 
$T_p = \frac{p(p+1)}{2}$ 
$T_{p+1} = \frac{(p+1)(p+2)}{2}$
$T_{p+1} - T_p = \frac{(p+1)(p+2)}{2} - \frac{p(p+1)}{2}$
$= \frac{(p+1)(p+2) - p(p+1)}{2}$
$= \frac{(p+1)( p + 2 - p)}{2}$
$= \frac{(p+1)(p+2-p)}{2}$
$= \frac{(p+1)2}{2}$
$=p+1$
Hence, $T_{n+1} = T_n + n+1$
where $T_{n+1} > T_n$ and $T_n, T_{n+1}$ are two consecutive triangular numbers.
$T_p>p$
- Opponent chooses, P
- We choose, W = $1^{T_p}0$ and $W \in T_p$
- Opponent chooses, $X = 1^a$ and $Y = 1^b$, where $XY = 1^a \cdot 1^b$
- Now, $1^{T_p}0=1^a1^b1^{T_p-(a+b)}0$
  - $X=1^a$
    $Y=1^b$
    and $|XY|\leq p$ therefore, $|Y| \leq p$
    therefore, $|Y|<p + 1$ or, $b<p+1$
therefore, $\#_1(W) = T_p$
let, $w' = XY^2Z = 1^a1^b1^b1^{T_p-(a+b)}0$
hence, $\#_1(W') =a+b+b+T_p-(a+b) = a+2b+T_p-a-b = T_p+b$
since, $b>0$ and $b<p+1$, $T_p<T_p+b< T_{p+1}$ where $T_{p+1}$ is the next triangular number.
Since, $T_p+b$ or $\#_1(W')$ is strictly between 2 triangualr number therefore $W' \notin L$

Hence We proved that, L is not regular.




qwdaqsdasdasdasda