# c 
Let, $T_p$ is $p^{th}$ number in the series of triangular number,i.e. $T_1 = 1, T_2 = 3, T_3 = 6,......T_n = n^{th}$ triangular number, where, $n\geq 1$
Now for an arbritary n =p and p+1 we get 2 consecutive triangular number, where $p<p+1$ and $T_p<T_{p+1}$
Now from the definition of triangular numbers,
$T_p = \frac{p(p+1)}{2}$ 
$T_{p+1} = \frac{(p+1)(p+2)}{2}$
$T_{p+1} - T_p = \frac{(p+1)(p+2)}{2} - \frac{p(p+1)}{2}$
$= \frac{(p+1)(p+2) - p(p+1)}{2}$
$= \frac{(p+1)( p + 2 - p)}{2}$
$= \frac{(p+1)(p+2-p)}{2}$
$= \frac{(p+1)2}{2}$
$=p+1$
Hence we can conclude that, $T_{n+1} = T_n + n+1$
where $T_{n+1} > T_n$ and $T_n, T_{n+1}$ are two consecutive triangular numbers.

__Pumping Lemma proof:__
- We pick language
L = {}
- Opponent picks a positive integer $p$
- We pick, $W = 1^{T_p}0$ where, $T_p = \frac{p(p+1)}{2}$ or, $T_p$ is the $p^{th}$ number in the triangular number series,  $W \in L$
- Opponent splits, $W = 1^{T_p}0 = XYZ$ with $|Y|>0$ and $|XY|\leq p$
- Since, $W$ contains only 1's, $XY$ also contain only 1's.
  So we can write, $X = 1^a$, $Y = 1^b$, $Z = 1^{T_p -(a+b)}$ for some $a \geq 0$ and $b > 0$
- We calculate, $XY^2Z = 1^a \cdot 1^b \cdot 1^b \cdot 1^{T_p -(a+b)} = 1^{a+b+b+T_p-(a+b)} = 1^{a+b+b+T_p-a-b} = 1^{T_p+b}$
- Since $b>0$, and $b\leq p$, it follows that, $T_p+b>T_p$ and $T_p+b \leq T_p+p$, 
  hence, $T_p+b < T_p + p + 1$, 
  $T_{p+1}$ is next triangular number to $T_p$, and we have shown that, $T_{p+1} = T_p+p+1$
  Hence, $T_p+b < T_{p+1}$, therefore, $T_p < T_p+b < T_{p+1}$
  So we can say that, $T_p+b$ is not a triangulae number, therefore, $\#_1(XY^2Z) = T_P+b$ is not a triangular number. 
  $\because$ $XY^0Z \notin L$ So, by the Pumping Lemma, L is not regular 

<!-- ---
- Opponent splits, $X = 1^a$ and $Y = 1^b$, where $XY = 1^a \cdot 1^b$
- Now, $1^{T_p}0=1^a1^b1^{T_p-(a+b)}0$
  - $X=1^a$
    $Y=1^b$
    and $|XY|\leq p$ therefore, $|Y| \leq p$
    therefore, $|Y|<p + 1$ or, $b<p+1$
therefore, $\#_1(W) = T_p$
let, $w' = XY^2Z = 1^a1^b1^b1^{T_p-(a+b)}0$
hence, $\#_1(W') =a+b+b+T_p-(a+b) = a+2b+T_p-a-b = T_p+b$
since, $b>0$ and $b<p+1$, $T_p<T_p+b< T_{p+1}$ where $T_{p+1}$ is the next triangular number.
Since, $T_p+b$ or $\#_1(W')$ is strictly between 2 triangualr number therefore $W' \notin L$

Hence We proved that, L is not regular. -->
