<center> <h1>A1</h1></center>

Contents
- [Q1](#q1)
  - [a](#a)
  - [b](#b)
- [Q2](#q2)
- [Q3](#q3)
  - [a](#a-1)
  - [b](#b-1)
  - [c](#c)
  - [d](#d)
  - [e](#e)
- [Q4](#q4)
  - [a](#a-2)
  - [b](#b-2)
  - [c](#c-1)
- [Q5](#q5)
- [Q6](#q6)
  - [a](#a-3)
  - [b](#b-3)
- [Q7](#q7)
  - [a](#a-4)
  - [b](#b-4)
  - [c](#c-2)
  - [d](#d-1)


## Q1
### a 
$w_1, w_2, w_4$ are in $L^*$

### b
$w_2, w_4$ are in $L^4$

<!-- $W_1$ and $W_3$ not found for $L^4$ -->
<!-- $W_3$ not found for $L^*$ -->

## Q2
<!-- :question: When calculating $L^*$ do we need to consider $L^0 = \epsilon$ in the shortlex order \ -->
1. $\epsilon$ 
2. 01
3. 010
4. 100
5. 0101
6. 01001
7. 01010
8. 01100
9. 10001
10. 010010
11. 010100
12. 010101
13. 100010
14. 100100
15. 0100101
16. 0101001
<!-- $\epsilon$, 01, 010, 100, 0101, 01001, 01010, 01100, 10001, 010010, 010100, 010101, 100010, 100100, 0100101, 0101001, 0101010, 0101100, 0110001 -->

## Q3
### a
$A^*B^*$ = $\{0\}^*\{1\}^*$ = Strings $0^n 1^m$ where $n, m \geq 0$ or Binary strings with zero or more 0's as prefix and zero or more 1's as suffix.
### b
$(AB)^* =(01)^*$ = Even length strings, with equal number of 0 and 1, starting with 0, ending in 1, and no consecutive same symbols.
### c
$(A \cap B)^*$ = set of empty string.
### d
$(A \cup B)^*AB$ = Binary string ending in 01.
### e
$(A^* \cup AB)^* - (BAB)^*$ = Binary String that don't end with 1 and no consecutive 1 in the string. 


## Q4
### a
 $G \times (H \cup K) = \{(a,1), (a, 2), (a, 3), (b,1), (b, 2), (b, 3)\}$
### b
$G \times (H \cap K) = \{a, b\} \times \{2\} = \{(a, 2), (b, 2)\}$
### c
$\mathscr{P}((G \times H) \cap (G \times K)) = \{\phi, \{(a, 2), (b, 2)\}, \{(a, 2)\}, \{(b, 2)\}\}$

## Q5
<!-- :boom: Try proof by cases
- Let's L is an arbitrary language. L = $\{x_1, x_2,......\}$ with length greater than 1.
- Now for strings $x_1$ and $x_2$ in L, by the given definition we  $x_1 \cdot x_2 \in L$. .......................(1)
  - If that's not true then L is not repeat avoiding. [case 1]
  - If that's true then **also** $x_1 \cdot x_2 \cdot x_1 \in L$. [case 2]
    - If that's not true then L is not repeat avoiding. [case 2.1]
    - If that's true then $x_1 \cdot x_2 \cdot x_1 \cdot x_2 \in L$. [case 2.2]  
      - If case 2.2 not true false then L is not repead [case 2.2.1]
      - If case 2.2 is true then proposition 1 is false, as $x_1 \cdot x_2 \in L$ and thus viewing all cases it  -->

We are given 2 propositions, 
**Proposition 1:** For all $W \in L$, we have $W\cdot W \notin L$
**Proposition 1:** For all $W_1, W_2 \in L$, such that $W_1 \not ={W_2}$ we have $W_1\cdot W_2 \in L$
A language is repeatn avoiding if both propostion (1) and (2) are true.

**Proof:**
Let L be an arbitrary language. where L = $\{x_1, x_2,......\}$ where $|L| > 1$.\
Let's consider 2 arbitrary strings $x_1$ and $x_2$, where $x_1, x_2\in L$\
Now We consider 2 cases, 
**Case 1**: $x_1 \cdot x_2 \notin L$\
If case 2 is true then L is not repeat avoiding as it fails to satisfy propostion (2).

**Case 2**: $x_1 \cdot x_2 \in L$ \
If case 1 is true then,
By proposition (2), $x_1 \cdot x_2 \cdot x_1$ should be in L, since $x_1\cdot x_2, x_1 \in L$\
Next we consider 2 more cases separately given Case 2 is true.
**case 2-a** $x_1 \cdot x_2 \cdot x_1 \notin l$\
If Case 2-a then L is not repeat avoiding, as it fails to satisfy propostion (2)

**case 2-b** $x_1 \cdot x_2 \cdot x_1 \in L$\
If case 2-b is true then, by propostion 2, $x_1 \cdot x_2 \cdot x_1 \cdot x_2 \in L$, since $x_1\cdot x_2 \cdot x_1, x_2 \in L$\
then it goes against propostion 1 
therefore for any language L it is not possible that both propostion (1) and (2) is true,\
therefore every language L with $|L| \geq 2$ is not repeat-avoiding
or No repeat-avoiding language exists.


## Q6
$S = \{00, 10, 010, 01001\}$
### a
We choose W = 010010, where $W \in S^*$

First picking the longest prefix 01001 from S,
We have ~~01001~~0, After this we are left 0, and $0 \notin S$, therefore for W = $010010$ the algorithm returns No, though the string $010010 \in S^*$

### b
We choose W = 01001, where $W \in S^*$

First picking the shortest prefix $W_1 \in S$ such that $W_1 \cdot y = 01001$

We picked 010, therefore the string becomes ~~010~~01, but $01 \notin S$ therefore we couldn't cross off all symbols of string W. Hence our algorithm output is No. But as we have showed before string $W \in S^*$


## Q7
### a
We are given 2 rules:
for any alphabet symbol x, define $x^R = x$ ............(1)
for any string W and any alphabet symbol x, define $(W_1\cdot W_2)^R = W_2^R\cdot W_1^R$ ............(2)

$W_1, W_2$ two strings $|W_1|\geq 1$ and $|W_2|= n$ where $n \geq 1$

**Base case**: For n = 1,
<!-- > :question: If $|W_2| = 1$, Can we apply $(W_1\cdot W_2)^R = W_2 \cdot W_1^R$ __DONE__ -->
Since $|W_2| = 1$, using rule 2
$(W_1\cdot W_2)^R = W_2 \cdot W_1^R$ 

**Induction Hypothesis**: For n = m, 
We assume, for $W_1, W_m$ where $W_1$ is an arbitrary string and $|W_m| = m$ 
$(W_1\cdot W_m)^R = W_m^R \cdot W_1^R$


**Inductive Step**
Now let's consider for $W_{m+1}$ where, $|W_{m+1}| = m + 1$,
We need to proof, **$(W_1 \cdot W_{m+1})^R = W_{m+1}^R \cdot W_1^R$**
Lets consider $W_{m+1} = W_m \cdot x$ and $|W_m| = m$, We can do that as $W_m$ is an arbritary string with length m and x is suffix symbol.

Now,
$(W_1\cdot W_{m+1})^R = (W_1\cdot W_m \cdot x)^R$
let, $W_1 \cdot W_m = W$
Then, $(W_1\cdot W_{m+1})^R = (W_1\cdot W_m \cdot x)^R = (W \cdot x)^R$
$\implies (W_1\cdot W_{m+1})^R = xW^R$ [$\because$ rule (2)]
$\implies (W_1\cdot W_{m+1})^R = x (W_1 \cdot W_m)^R$ By replacing value of $W$ with $W_1 \cdot W_m$ 

**Using our induction hypothesis**, since $(W_1\cdot W_m)^R = W_m^R \cdot W_1^R$
$\implies (W_1\cdot W_{m+1})^R = x\cdot W_m^R \cdot W_1^R $ ............(3)

Now,
$(W_m \cdot x)^R = x \cdot W_m^R$ [from rule (2)]
$\implies W_{m+1}^R = x \cdot W_m^R$ .................(4)


Hence, from (3) and (4) we have, 
$(W_1\cdot W_{m+1})^R = W_{m+1}^R \cdot W_1^R $

Therefore by mathematical induction we have proved that, for all non-empty strings $W_1, W_2$, we have $(W_1 \cdot W_2)^R = W_2^R \cdot W_1^R$



### b

**Base Case** k = 2
$(W_1 \cdot W_2)^R = W_2^R \cdot W_1^R$ [from the answer of **7(a)**]

**Induction Hypothesis**
We assume for k = m
$(W_1 \cdot W_2 \cdot \cdot \cdot W_m)^R = W_m^R \cdot \cdot \cdot W_2^R \cdot W_1^R$

**Inductive Step**
__We will prove that__, for k = m+1,  $(W_1 \cdot W_2 \cdot \cdot \cdot W_m \cdot W_{m+1})^R = W_{m+1}^R \cdot W_m^R \cdot \cdot \cdot W_2^R \cdot W_1^R$

L.H.S = $(W_1 \cdot W_2 \cdot \cdot \cdot W_k \cdot W_{k+1})^R$
= $(W \cdot W_{k+1})^R$, where $W = W_1 \cdot W_2 \cdot \cdot \cdot W_k$
= $W_{k+1}^R \cdot W^R$ [from the answer of **7(a)**]
= $W_{k+1}^R \cdot (W_1 \cdot W_2 \cdot \cdot \cdot W_k)^R$ [replacing W with it's value]
= $W_{k+1}^R \cdot W_k^R \cdot \cdot \cdot W_2^R \cdot W_1^R$ [Applying induction hypothesis]
= R.H.S
Therefore by mathematical induction we have proved that, For all $k \geq 2$, for all k non-empty strings $W_1,......W_k$, we have $(W_1 \cdot \cdot \cdot \cdot W_k)^R = W_k^R \cdot \cdot \cdot W_1^R$
### c
<!-- :question: Since k has no upper limit, kinda like limit can we use Induction?
:question: Is **x** **non-empty**?
:question: We can't use the definition of reverse, but can we use the definition of palindrome? that is, **if $X$ is a palindrome then $X^R = X$**
:question: For a power of string, can we say **$x^m \cdot x = x \cdot x^m$**
:question: Can we use **$|X^R| == |X|$** -->

We will prove, If $X$ is a palindrome, then $X^n$ is a palindrome.

If $X$ is a palindrome, 
__Base Case__: for n = 1,

$X^n  = X$, [using the definition of palindrome]
therefore the statement is true for n = 1

 __Induction Hypothesis__ for n = m
 Assume, the statement, If $X$ is a palindrome, then $X^m$ is also a palindrome, is true.

 __induction step__ 
 for n = m+1, We need to prove,  the statement is true.

 $X^{m+1} = X^m \cdot X$
 $\therefore (X^{m+1})^R = (X^m \cdot X)^R = X^R \cdot (X^m)^R$ [from the answer of **7(a)**]
 $\therefore (X^{m+1})^R = X \cdot X^m$ [__Since $X$ is a plaindome and using Induction hypothesis__]
 $\therefore (X^{m+1})^R = X^{m+1}$
 Hence $x^{m+1}$ is a palindrome.

Therefore by mathematical induction we have proved that, for all string $X$ and all $n \geq 1$, if $X$ is a palindrome then $X^n$ is a palindrome. 

### d
For this we will proof contrapositive of the statement,
**Contrapositive**: If $X$ is not a palindrome then $X^n$ is not a palindrome.
__Base case__
for n = 1,
$X^1 = X$, hence if $X$ is not a palindrome then $X \not ={X^R}$
therefpre the statement is true for base case. 

__Induction Hypothesis__ for n = m
Assume if $X$ is not a palindrome then, $X^m$ is not a palindrome 

__induction step__ for n = m+1,
$X^{m+1} = X^m \cdot X$
$\therefore (X^{m+1})^R = (X^m \cdot X)^R = X^R \cdot (X^m)^R$ [from the answer of **7(a)**]

Now $X^{m + 1} = X^m \cdot X = X \cdot X^m$
Since $X$ is not a palindrome then $X \not ={X^R}$ but $|X| = |X^R|$

Therefore between strings $X^R \cdot (X^m)^R$ and $X \cdot X^m$ the prefix is same length and are not equal therefore the 2 string can not be equal. therefore , $X^{m+1} \not ={(X^{m+1})^R}$ hence $X^{m+1}$ is not a palindrome.

Therefore by mathematical induction we have proved that, 
for all strings $X$ and all $n\geq 1$, If $X$ is not a palindrome then $X^n$ is not a palindrome
i.e. if $X^n$ is a palindrome, then $X$ is a palindrome.
<!-- Between  $x^R \cdot (x^m)^R$ and $x \cdot x^m$ the suffix (x^m)^R and x^m is not same and it has same length, therefire we can conclude that $x^R \cdot (x^m)^R \not ={x \cdot x^m}$ or $x^R \cdot (x^m)^R \not =x^{m+1}$
hence $x^{m+1} \not ={(x^{m+1})^R}$, therfore $x^{m+1}$ is not a palindrome. -->